Big refactor preparing local read lemmas:
* Add zero-sized read/write semantics (these do not affect the tree, and do not require the tag to exist)
* Split up steps_refl and steps_opt into more manageable files
* Create an early_proofmode that is just the old proofmode but with less things additionally `Require Export`ed
* Prepare `steps_local.v`
* Slightly modify the simulation relation to ban empty local heaplets.

theories/tree_borrows/defs.v
@@ -79,10 +79,10 @@ Arguments same_blocks / _ _.
 (* FIXME: forall blk, (exists l, is_Some (hp !! (blk, l))) <-> is_Some (trs !! blk). *)
 
 Definition root_invariant blk it (shp : mem) :=
-  it.(iprot) = None ∧
-  ∀ off, match item_lookup it off with
-    mkPerm PermInit Active => is_Some (shp !! (blk, off))
-  | mkPerm PermLazy Disabled => shp !! (blk, off) = None
+  it.(iprot) = None ∧ it.(initp) = Disabled ∧
+  ∀ off, match it.(iperm) !! off with
+    Some (mkPerm PermInit Active) => is_Some (shp !! (blk, off))
+  | Some (mkPerm PermLazy Disabled) | None => shp !! (blk, off) = None
   | _ => False end.
 
 
