theories/tree_borrows/step_laws/steps_local.v
@@ -22,17 +22,87 @@ Implicit Types l : loc.
 Implicit Types f : fname.
 
 
+(** ** Copy lemmas *)
+Lemma target_copy_local v_t sz l t Ψ :
+  length v_t = sz →
+  t $$ tk_local -∗
+  l ↦t∗[tk_local]{t} v_t -∗
+  (l ↦t∗[tk_local]{t} v_t -∗ t $$ tk_local -∗ target_red #v_t Ψ)%E -∗
+  target_red (Copy (Place l t sz)) Ψ.
+Proof.
+  iIntros (Hlen) "Htag Ht Hsim".
+  iApply target_red_lift_base_step. iIntros (P_t σ_t P_s σ_s ?) "(HP_t & HP_s & Hbor)".
+  iPoseProof (bor_interp_get_state_wf with "Hbor") as "[%Hwf_t %]".
+  iModIntro. iDestruct "Hbor" as "(%M_call & %M_tag & %M_t & %M_s & Hbor)".
+  iPoseProof (bor_interp_readN_target_local with "Hbor Ht Htag") as "(%Hd & %Hstack)".
+  rewrite Hlen in Hd Hstack.
+  have READ_t : read_mem l sz σ_t.(shp) = Some v_t.
+  { apply read_mem_values'; done. }
+  eapply read_mem_values in READ_t as HX. destruct HX as (Hv_t_len & _).
+  have Eq_trs : apply_within_trees (memory_access AccessRead σ_t.(scs) t (l.2, sz)) l.1 σ_t.(strs) = Some σ_t.(strs).
+  { eapply local_access_preserves_unchanged. 1: done. 1: exact Hv_t_len. 2: apply Hd. 2: done.
+  (*
+  have Eq_stk : memory_read σ_t.(sst) σ_t.(scs) l (Tagged t) (tsize T) = Some σ_t.(sst).
+  { apply memory_read_access1. intros i Hi.
+    specialize (Hstack i Hi). eexists; split; first done. eapply bor_state_own_access1_read; done. }
+  iSplitR.
+  { iPureIntro. do 3 eexists; eapply copy_base_step'; [done | done | eauto ]. }
+  iIntros (e_t' efs_t σ_t') "%Hhead".
+  specialize (head_copy_inv _ _ _ _ _ _ _ _ Hhead) as [-> [(v_t' & α' & READ & ACC & -> & ->) | (_ & Hfail & _)]]; last congruence.
+  rewrite READ in READ_t. simplify_eq.
+  iModIntro. iSplitR; first done.
+  iFrame "HP_t HP_s".
+  iSplitL "Hbor"; last iApply ("Hsim" with "Ht Htag").
+  destruct σ_t; done.
+Qed. *) Admitted.
 (*
-Lemma target_write_local v_t v_t' T l t Ψ :
-  length v_t = tsize T →
-  length v_t' = tsize T →
+Lemma source_copy_local v_s T l t Ψ π :
+  length v_s = tsize T →
+  t $$ tk_local -∗
+  l ↦s∗[tk_local]{t} v_s -∗
+  (l ↦s∗[tk_local]{t} v_s -∗ t $$ tk_local -∗ source_red #v_s π Ψ)%E -∗
+  source_red (Copy (Place l (Tagged t) T)) π Ψ.
+Proof.
+  iIntros (Hlen) "Htag Hs Hsim".
+  iApply source_red_lift_base_step. iIntros (P_t σ_t P_s σ_s ??) "[(HP_t & HP_s & Hbor) _]".
+  iModIntro.
+  iPoseProof (bor_interp_get_state_wf with "Hbor") as "[% %Hwf_s]".
+  iPoseProof (bor_interp_readN_source_local with "Hbor Hs Htag") as "(%Hd & %Hstack)".
+  rewrite Hlen in Hd Hstack.
+  have READ_s : read_mem l (tsize T) σ_s.(shp) = Some v_s.
+  { apply read_mem_values'; done. }
+  have Eq_stk : memory_read σ_s.(sst) σ_s.(scs) l (Tagged t) (tsize T) = Some σ_s.(sst).
+  { apply memory_read_access1. intros i Hi.
+    specialize (Hstack i Hi). eexists; split; first done. eapply bor_state_own_access1_read; done. }
+  assert (base_reducible P_s (Copy (Place l (Tagged t) T)) σ_s) as (e_s' & σ_s' & efs & Hhead).
+  { do 3 eexists; eapply copy_base_step'; [done | done | eauto ]. }
+  iExists e_s', σ_s'.
+  specialize (head_copy_inv _ _ _ _ _ _ _ _ Hhead) as [-> [(v_t' & α' & READ & ACC & -> & ->) | (_ & Hfail & _)]]; last congruence.
+  rewrite READ in READ_s. simplify_eq.
+  iFrame "HP_t HP_s". iSplitR; first done.
+  iSplitL "Hbor"; last by iApply ("Hsim" with "Hs Htag"). iModIntro.
+  by destruct σ_s.
+Qed.
+
+(** ** Write *)
+
+
+
+Lemma target_write_local v_t v_t' sz l t Ψ :
+  length v_t = sz →
+  length v_t' = sz →
   t $$ tk_local -∗
   l ↦t∗[tk_local]{t} v_t -∗
   (l ↦t∗[tk_local]{t} v_t' -∗ t $$ tk_local -∗ target_red #[☠] Ψ)%E -∗
-  target_red (Write (Place l (Tagged t) T) #v_t') Ψ.
+  target_red (Write (Place l t sz) #v_t') Ψ.
 Proof.
   iIntros (Hlen Hlen') "Htag Ht Hsim".
   iApply target_red_lift_base_step. iIntros (P_t σ_t P_s σ_s ?) "(HP_t & HP_s & Hbor)".
+  iDestruct "Hbor" as "(%M_call & %M_tag & %M_t & %M_s & (Hc & Htag_auth & Htag_t_auth & Htag_s_auth) & Hpub_cid & #Hsrel & %Hcall_interp & %Htag_interp & _ & _)".
+  
+  
+
+
   iPoseProof (bor_interp_readN_target_local with "Hbor Ht Htag") as "(%Hd & %Hstack)".
   iMod (bor_interp_writeN_target_local _ _ _ _ _ v_t' with "Hbor Ht Htag []") as "(Hbor & Ht & Htag)";
     first (iPureIntro; lia).
@@ -85,63 +155,6 @@ Proof.
   done.
 Qed.
 
-(** ** Copy lemmas *)
-Lemma target_copy_local v_t T l t Ψ :
-  length v_t = tsize T →
-  t $$ tk_local -∗
-  l ↦t∗[tk_local]{t} v_t -∗
-  (l ↦t∗[tk_local]{t} v_t -∗ t $$ tk_local -∗ target_red #v_t Ψ)%E -∗
-  target_red (Copy (Place l (Tagged t) T)) Ψ.
-Proof.
-  iIntros (Hlen) "Htag Ht Hsim".
-  iApply target_red_lift_base_step. iIntros (P_t σ_t P_s σ_s ?) "(HP_t & HP_s & Hbor)".
-  iModIntro.
-  iPoseProof (bor_interp_readN_target_local with "Hbor Ht Htag") as "(%Hd & %Hstack)".
-  rewrite Hlen in Hd Hstack.
-  have READ_t : read_mem l (tsize T) σ_t.(shp) = Some v_t.
-  { apply read_mem_values'; done. }
-  iPoseProof (bor_interp_get_state_wf with "Hbor") as "[%Hwf_t %]".
-  have Eq_stk : memory_read σ_t.(sst) σ_t.(scs) l (Tagged t) (tsize T) = Some σ_t.(sst).
-  { apply memory_read_access1. intros i Hi.
-    specialize (Hstack i Hi). eexists; split; first done. eapply bor_state_own_access1_read; done. }
-  iSplitR.
-  { iPureIntro. do 3 eexists; eapply copy_base_step'; [done | done | eauto ]. }
-  iIntros (e_t' efs_t σ_t') "%Hhead".
-  specialize (head_copy_inv _ _ _ _ _ _ _ _ Hhead) as [-> [(v_t' & α' & READ & ACC & -> & ->) | (_ & Hfail & _)]]; last congruence.
-  rewrite READ in READ_t. simplify_eq.
-  iModIntro. iSplitR; first done.
-  iFrame "HP_t HP_s".
-  iSplitL "Hbor"; last iApply ("Hsim" with "Ht Htag").
-  destruct σ_t; done.
-Qed.
-
-Lemma source_copy_local v_s T l t Ψ π :
-  length v_s = tsize T →
-  t $$ tk_local -∗
-  l ↦s∗[tk_local]{t} v_s -∗
-  (l ↦s∗[tk_local]{t} v_s -∗ t $$ tk_local -∗ source_red #v_s π Ψ)%E -∗
-  source_red (Copy (Place l (Tagged t) T)) π Ψ.
-Proof.
-  iIntros (Hlen) "Htag Hs Hsim".
-  iApply source_red_lift_base_step. iIntros (P_t σ_t P_s σ_s ??) "[(HP_t & HP_s & Hbor) _]".
-  iModIntro.
-  iPoseProof (bor_interp_get_state_wf with "Hbor") as "[% %Hwf_s]".
-  iPoseProof (bor_interp_readN_source_local with "Hbor Hs Htag") as "(%Hd & %Hstack)".
-  rewrite Hlen in Hd Hstack.
-  have READ_s : read_mem l (tsize T) σ_s.(shp) = Some v_s.
-  { apply read_mem_values'; done. }
-  have Eq_stk : memory_read σ_s.(sst) σ_s.(scs) l (Tagged t) (tsize T) = Some σ_s.(sst).
-  { apply memory_read_access1. intros i Hi.
-    specialize (Hstack i Hi). eexists; split; first done. eapply bor_state_own_access1_read; done. }
-  assert (base_reducible P_s (Copy (Place l (Tagged t) T)) σ_s) as (e_s' & σ_s' & efs & Hhead).
-  { do 3 eexists; eapply copy_base_step'; [done | done | eauto ]. }
-  iExists e_s', σ_s'.
-  specialize (head_copy_inv _ _ _ _ _ _ _ _ Hhead) as [-> [(v_t' & α' & READ & ACC & -> & ->) | (_ & Hfail & _)]]; last congruence.
-  rewrite READ in READ_s. simplify_eq.
-  iFrame "HP_t HP_s". iSplitR; first done.
-  iSplitL "Hbor"; last by iApply ("Hsim" with "Hs Htag"). iModIntro.
-  by destruct σ_s.
-Qed.
 
 (** ** Alloc *)
 Lemma sim_alloc_local T Φ π :
